theories/generic/utp_types.thy
@@ -12,35 +12,35 @@ begin
 
 text {* This theory defines type synonyms for the various semantic domains. *}
 
-types 'TYPE VAR =
+type_synonym 'TYPE VAR =
   "NAME \<times> 'TYPE"
 
-types 'TYPE ALPHABET =
+type_synonym 'TYPE ALPHABET =
   "('TYPE VAR) set"
 
-types ('VALUE, 'TYPE) BINDING =
+type_synonym ('VALUE, 'TYPE) BINDING =
   "('TYPE VAR) \<Rightarrow> 'VALUE"
 
-types ('VALUE, 'TYPE) BINDING_SET =
+type_synonym ('VALUE, 'TYPE) BINDING_SET =
   "('VALUE, 'TYPE) BINDING set"
 
-types ('VALUE, 'TYPE) BINDING_BFUN =
+type_synonym ('VALUE, 'TYPE) BINDING_BFUN =
   "('VALUE, 'TYPE) BINDING \<Rightarrow> bool"
 
-types ('VALUE, 'TYPE) BINDING_FUN =
+type_synonym ('VALUE, 'TYPE) BINDING_FUN =
   "('VALUE, 'TYPE) BINDING \<Rightarrow> 'VALUE"
 
-types ('VALUE, 'TYPE) PREDICATE =
+type_synonym ('VALUE, 'TYPE) PREDICATE =
   "('VALUE, 'TYPE) BINDING_SET"
 
-types ('VALUE, 'TYPE) FUNCTION =
+type_synonym ('VALUE, 'TYPE) FUNCTION =
   "('VALUE, 'TYPE) PREDICATE \<Rightarrow>
    ('VALUE, 'TYPE) PREDICATE"
 
-types ('VALUE, 'TYPE) ALPHA_PREDICATE =
+type_synonym ('VALUE, 'TYPE) ALPHA_PREDICATE =
   "('TYPE ALPHABET) \<times> ('VALUE, 'TYPE) PREDICATE"
 
-types ('VALUE, 'TYPE) ALPHA_FUNCTION =
+type_synonym ('VALUE, 'TYPE) ALPHA_FUNCTION =
   "('VALUE, 'TYPE) ALPHA_PREDICATE \<Rightarrow>
    ('VALUE, 'TYPE) ALPHA_PREDICATE"
 end
